denotational/Vectors.v
@@ -1,31 +1,78 @@
 From Coq Require Import
      Vector
+     Fin
      Program.Equality.
 
-From Coq Require Fin.
+From Coq Require List.
 
 Import VectorNotations.
+
 From Equations Require Import Equations.
 
 From DSL Require Import Agent.
 
 Module VectorUtils.
 
-  Definition vec n T := Vector.t T n.
+  Declare Scope fin_vector_scope.
 
-  Definition fin := Fin.t.
+  Notation vec n T := (Vector.t T n).
+  Notation fin := Fin.t.
 
-  Import Fin.
   Equations vector_remove{A n}(v: vec (S n) A)(i: fin (S n)) : vec n A by wf n lt :=
     vector_remove (h :: h' :: ts) (FS (FS j)) := h :: (vector_remove (h' :: ts) (FS j));
     vector_remove (h :: h' :: ts) (FS F1) := h :: ts;
     vector_remove (h :: h' :: ts) F1 := h' :: ts;
     vector_remove (h::nil) F1 := @nil A.
                                                    
-  Equations vector_replace{A n}(v: vec (S n) A)(i: fin (S n))(a: A): vec (S n) A by wf n lt :=
+  Equations vector_replace{A n}(v: vec n A)(i: fin n)(a: A): vec n A by wf n lt :=
+    vector_replace [] _ _ := [];
     vector_replace (h :: h' :: ts) (FS (FS j)) a := h :: (vector_replace (h' :: ts) (FS j) a);
     vector_replace (h :: h' :: ts) (FS F1) a := h :: a :: ts;
     vector_replace (h :: h' :: ts) F1 a := a :: h' :: ts;
-    vector_replace (h::nil) F1 a := [a].
+    vector_replace [h] F1 a := [a].
 
+  Notation "v '@' i ':=' a" := (vector_replace v i a) (at level 80): fin_vector_scope.
+  Notation "v '$' i" := (nth v i) (at level 80): fin_vector_scope.
+  Notation "v '--' i" := (vector_remove v i) (at level 80): fin_vector_scope.
+
+  (** Vector utils *)
+  Equations forallb {A}{m: nat}(f: A -> bool)(a: vec m A): bool :=
+    forallb _ [] := true;
+    forallb f (h :: ts) := andb (f h) (forallb f ts).
+
+  Lemma forall_reflect: forall A (m: nat)(f: A -> bool) (l: vec m A),
+      forallb f l = true <-> Forall (fun x => f x = true) l.
+  Proof.
+    intros A m f l. 
+    split; intros.
+    - dependent induction l.
+      + econstructor.
+      + econstructor; replace (forallb f (h :: l)) with
+            (andb (f h) (forallb f l)) in H by reflexivity;
+          apply andb_prop in H;
+          destruct H.
+        * exact H.
+        * apply IHl; assumption.
+    - dependent induction H.
+      + reflexivity.
+      + replace (forallb f (x :: v)) with
+          (andb (f x) (forallb f v)) by reflexivity.
+        apply andb_true_intro; split; assumption.
+  Defined.
+
+  
+  Fixpoint last{A}(l: list A): option A :=
+    match l with
+    | List.nil => None
+    | List.cons h List.nil => Some h
+    | List.cons h ts => last ts
+    end.
+
+  Fixpoint init{A}(l: list A): list A :=
+    match l with
+    | List.nil => List.nil
+    | List.cons h List.nil => List.nil
+    | List.cons h ts => List.cons h (init ts)
+    end.
+  
 End VectorUtils.
